src/rocq/Theory/ContainsUB.v
@@ -417,7 +417,7 @@ Section refine_OOM_h_lemmas.
   Hint Resolve interp_PropT__mono : paco.
 
   (* Only the <- direction is true *)
-  Global Instance proper_refine_OOM_h
+  (* Global Instance proper_refine_OOM_h
     {R} {RR : relation R} : Proper (@refine_OOM_h Eff _ _ RR ==> flip impl) contains_UB.
     unfold Proper, respectful.
     intros x y EQ UB; revert x EQ.
@@ -567,5 +567,5 @@ Section refine_OOM_h_lemmas.
     intros R RR x y UB REF.
     rewrite REF.
     eauto.
-  Qed.
+  Qed. *)
 End refine_OOM_h_lemmas.
